

## Homework 2.

### Theory question

**Question 1. Derive the normal equations and the  $\hat{\beta}$  from the multivariate version of the multiple regression likelihood**

$$\frac{\partial \ell(\beta, \sigma^2)}{\partial \beta} = \frac{\partial}{\partial \beta} \left[ -\frac{n}{2} \log(2\pi\sigma^2) - \frac{1}{2\sigma^2} (Y - X\beta)'(Y - X\beta) \right]$$

Since  $-\frac{n}{2} \log(2\pi\sigma^2)$  is constant with respect to  $\beta$ :

$$\frac{\partial \ell}{\partial \beta} = 0 - \frac{1}{2\sigma^2} \frac{\partial}{\partial \beta} [(Y - X\beta)'(Y - X\beta)]$$

Let  $Q = (Y - X\beta)'(Y - X\beta) = Y'Y - 2\beta'X'Y + \beta'X'X\beta$ . Then:

$$\frac{\partial Q}{\partial \beta} = -2X'Y + 2X'X\beta$$

Set the derivative to zero:

$$\frac{1}{\sigma^2} (2X'Y - 2X'X\beta) = 0$$

$$X'X\beta = X'Y$$

$$\hat{\beta}_{MLE} = (X'X)^{-1}X'Y$$

**Question 2. Demonstrate that  $\hat{\beta}$  is an unbiased estimator of  $\beta$**

$$\begin{aligned}Y &= X\beta + \epsilon \\ \hat{\beta} &= (X'X)^{-1}X'Y \\ \hat{\beta} &= (X'X)^{-1}X'(X\beta + \epsilon) \\ \hat{\beta} &= (X'X)^{-1}X'(X\beta) + (X'X)^{-1}X'(\epsilon) \\ \hat{\beta} &= (X'X)^{-1}(X'X)\beta + (X'X)^{-1}X'(\epsilon) \\ \hat{\beta} &= \beta + (X'X)^{-1}X'(\epsilon) \\ E(\hat{\beta}) &= \beta + E((X'X)^{-1}X'(\epsilon)) \\ E(\hat{\beta}) &= \beta + (X'X)^{-1}X' E(\epsilon) \\ E(\epsilon) &= 0 \quad (\text{by assumption})\end{aligned}$$

$$\boxed{E(\hat{\beta}) = \beta}$$

**Question 3. Demonstrate that  $\hat{\beta}$  follows a multivariate normal distribution**

$$\begin{aligned}\text{Cov}(\hat{\beta}) &= \text{Cov}((X'X)^{-1}X'\epsilon) \\ &= (X'X)^{-1}X' \cdot \text{Cov}(\epsilon) \cdot [(X'X)^{-1}X']' \\ &= (X'X)^{-1}X' \cdot (\sigma^2 I_n) \cdot X(X'X)^{-1} \\ &= (\sigma^2 I_n)(X'X)^{-1}X'X(X'X)^{-1} \\ &= (\sigma^2 I_n)(X'X)^{-1}\end{aligned}$$

$$E(\hat{\beta}) = \beta \quad \text{Cov}(\hat{\beta}) = (\sigma^2 I_n)(X'X)^{-1}$$

A **linear transformation** of a multivariate normal is also a **multivariate normal**, and

$$\hat{\beta} = A + C(\epsilon)$$

$$\hat{\beta} = \beta + (X'X)^{-1}X'\epsilon$$

Therefore

Since  $\epsilon \sim N(0, \sigma^2 I_n)$  and  $\hat{\beta}$  is a linear transformation of  $\epsilon$ , it follows that:

$$\hat{\beta} \sim N(\beta, \sigma^2(X'X)^{-1})$$